don't forget to squash

workloads/Coq/BST/Src/Spec.v
@@ -3,6 +3,31 @@ From QuickChick Require Import QuickChick. Import QcNotation.
 From Coq Require Import Bool ZArith List. Import ListNotations.
 From BST Require Import Impl.
 
+
+Class Implies (A B : Type) := implies : A -> B -> option bool.
+Notation "A -=> B" := (implies A B) (at level 199, left associativity).
+
+#[global] Instance impliesOO : Implies (option bool) (option bool) :=
+    fun p1 p2 => 
+        match p1 with
+        | None | Some false => None
+        | Some true => p2
+        end.
+
+#[global] Instance impliesBB : Implies bool bool := 
+    fun p1 p2 => 
+        impliesOO (Some p1) (Some p2).
+
+#[global] Instance impliesOB : Implies (option bool) bool := 
+    fun p1 p2 =>
+        impliesOO p1 (Some p2).
+
+#[global] Instance impliesBO : Implies bool (option bool) :=
+    fun p1 p2 =>
+        impliesOO (Some p1) p2.
+
+
+
 Fixpoint keys (t: Tree): list nat :=
   match t with
   | E => nil
@@ -66,21 +91,21 @@ Definition prop_UnionValid (t1: Tree) (t2: Tree) :=
 
 Definition prop_InsertPost (t: Tree) (k: nat) (k': nat) (v: nat) :=
   isBST t
-    -=> (find k' (insert k v t) ==? if k =? k' then Some v else find k' t).
+    -=> (find k' (insert k v t) = if k =? k' then Some v else find k' t)?.
 
 Definition prop_DeletePost (t: Tree) (k: nat) (k': nat) :=
   isBST t
-    -=> (find k' (delete k t) ==? if k =? k' then None else find k' t).
+    -=> (find k' (delete k t) = if k =? k' then None else find k' t)?.
 
 Definition prop_UnionPost (t: Tree) (t': Tree) (k: nat) :=
   isBST t
     -=>
     (let lhs := find k (union t t') in
     match (find k t) with
-    | Some rhs => lhs ==? (Some rhs)
+    | Some rhs => (lhs = (Some rhs))?
     | None => match (find k t') with
-            | Some rhs => lhs ==? (Some rhs)
-            | None => lhs ==? None
+            | Some rhs => (lhs = (Some rhs))?
+            | None => (lhs = None)?
             end
     end).
 
@@ -115,12 +140,12 @@ Fixpoint sorted (l: list (nat * nat)): bool :=
 
 Definition prop_InsertModel (t: Tree) (k: nat) (v: nat) :=
   isBST t
-    -=> (toList (insert k v t) ==? L_insert (k, v) (deleteKey k (toList t))).
+    -=> (toList (insert k v t) = L_insert (k, v) (deleteKey k (toList t)))?.
 
 
 Definition prop_DeleteModel (t: Tree) (k: nat) :=
   isBST t
-    -=> Some(toList (delete k t) ==? deleteKey k (toList t)).
+    -=> Some((toList (delete k t) = deleteKey k (toList t))?).
 
 
 Fixpoint L_sort (l: list (nat * nat)): list (nat * nat) :=
@@ -152,7 +177,7 @@ Fixpoint L_unionBy (f: nat -> nat -> nat) (l1: list (nat * nat)) (l2: list (nat 
 
 Definition prop_UnionModel (t: Tree) (t': Tree) :=
   (isBST t && isBST t')
-    -=> (toList (union t t') ==? L_sort (L_unionBy (fun x y => x) (toList t) (toList t'))).
+    -=> (toList (union t t') = L_sort (L_unionBy (fun x y => x) (toList t) (toList t')))?.
 
 
 (* ---------- *)
