workloads/Coq/STLC/Strategies/NewGenerator.v
@@ -1,0 +1,262 @@
+ 
+From QuickChick Require Import QuickChick. Import QcNotation.
+From Coq Require Import Bool ZArith List. Import ListNotations.
+From ExtLib Require Import Monad.
+From ExtLib.Data.Monads Require Import OptionMonad.
+Import MonadNotation.
+
+From STLC Require Import Impl Spec.
+
+Derive (Arbitrary) for Typ.
+Derive (Arbitrary) for Expr.
+
+Inductive bind : Ctx -> nat -> Typ -> Prop :=
+| BindNow   : forall tau env, bind (tau :: env) 0 tau
+| BindLater : forall tau tau' x env,
+    bind env x tau -> bind (tau' :: env) (S x) tau.
+
+Inductive typing (G : Ctx) : Expr -> Typ -> Prop :=
+| TyVar :
+    forall x T,
+      bind G x T ->
+      typing G (Var x) T
+| TyBool :
+    forall b,
+      typing G (Bool b) TBool
+| TyAbs :
+    forall e T1 T2,
+      typing (T1 :: G) e T2 ->
+      typing G (Abs T1 e) (TFun T1 T2)
+| TyApp :
+    forall e1 e2 T1 T2,
+      typing G e1 (TFun T1 T2) ->
+      typing G e2 T1 ->
+      typing G (App e1 e2) T2.
+
+
+(* Look up in list of backtrack weights *)
+Fixpoint get {a: Type} (l : list (nat * a)) (target_key : nat) (default : a): a :=
+  match l with
+  | [] =>
+    (* This branch should never return *)
+    default
+  | (key, value) :: l' =>
+    if Nat.eqb key target_key then
+       value
+    else get l' target_key default
+  end.
+
+
+#[export] Instance dec_type (t1 t2 : Typ) : Dec (t1 = t2).
+Proof. dec_eq. Defined.
+Derive Arbitrary for Typ.
+
+Fixpoint genVar' (ctx: Ctx) (t: Typ) (p: nat) (r: list nat) : list nat :=
+  match ctx with
+  | nil => r
+  | t'::ctx' =>
+      if t = t'? then genVar' ctx' t (p + 1) (p :: r)
+      else genVar' ctx' t (p + 1) r
+  end.
+
+Fixpoint genZero env tau : G (option Expr) :=
+  match tau with
+  | TBool =>
+      bindGen arbitrary
+              (fun b : bool =>
+                 returnGen (Some (Bool b)))
+  | TFun T1 T2 => 
+      bindOpt
+        (genZero (T1 :: env) T2)
+        (fun e : Expr =>
+           returnGen (Some (Abs T1 e)))
+  end.
+
+Fixpoint genTyp (s: nat) : G Typ :=
+  match s with
+  | 0 => ret TBool
+  | S s' =>
+    let '(boolWeight, funWeight) :=
+      get
+      [
+        (1, (581, 1000-581));
+        (2, (807, 1000-807))
+      ]
+      s
+      (0, 0) in
+    freq [
+      (boolWeight, ret (TBool))
+      ;
+      (funWeight,
+          t1 <- genTyp s';;
+          t2 <- genTyp s';;
+          ret (TFun t1 t2))
+    ]
+  end.
+  
+Fixpoint genExpr env tau (sz: nat) : G (option Expr) :=
+  match sz with
+  | 0 =>
+      backtrack
+        [(1, oneOf_ (ret None) (map (fun x => returnGen (Some (Var x))) (genVar' env tau 0 [])))
+        ;(1, genZero env tau)] 
+  | S sz' =>
+      let '(val_weight, app_weight, var_weight) :=
+        get
+          [
+            (1, (40, 662, 722));
+            (2, (126, 544, 717));
+            (3, (89, 815, 269));
+            (4, (465, 589, 432));
+            (5, (32, 800, 500))
+          ]
+          sz
+          (0, 0 ,0) in
+      backtrack
+        [(var_weight, oneOf_ (ret None) (map (fun x => returnGen (Some (Var x))) (genVar' env tau 0 [])))
+         ;
+        (app_weight,
+          bindGen (genTyp 2)
+                  (fun T1 : Typ =>
+          bindOpt
+            (genExpr env (TFun T1 tau) sz')
+            (fun e1 : Expr =>
+          bindOpt
+            (genExpr env T1 sz')
+            (fun e2 : Expr =>
+               returnGen (Some (App e1 e2))))))
+         ; 
+         (val_weight,
+           match tau with
+           | TBool =>
+               bindGen arbitrary
+                       (fun b : bool =>
+                          returnGen (Some (Bool b)))
+           | TFun T1 T2 =>
+               bindOpt
+                 (genExpr (T1 :: env) T2 sz')
+                    (fun e : Expr =>
+                     returnGen (Some (Abs T1 e)))
+              end)]
+  end.
+
+Definition gSized := 
+    typ <- arbitrary ;;
+    genExpr [] typ 5.
+
+
+Definition test_prop_SinglePreserve :=
+  forAllMaybe gSized (fun (e: Expr) =>
+    prop_SinglePreserve e).
+
+(*! QuickChick test_prop_SinglePreserve. *)
+  
+Definition test_prop_MultiPreserve :=
+  forAllMaybe gSized (fun (e: Expr) =>
+    prop_MultiPreserve e).
+  
+(*! QuickChick test_prop_MultiPreserve. *)
+
+(*
+Derive (Arbitrary) for Typ.
+
+
+(* Fixpoint genTyp (s: nat) : G Typ :=
+  match s with
+  | 0 => ret TBool
+  | S s' => oneOf [
+    t1 <- genTyp s' ;;
+    t2 <- genTyp s' ;;
+    ret (TFun t1 t2) ;
+    ret TBool
+    ]
+  end.
+   *)
+
+(* #[export] Instance genArbitrary : GenSized Typ :=
+{|
+ arbitrarySized x := genTyp x
+|}. *)
+
+Definition genTyp (s: nat) : G Typ := arbitrary.
+
+Fixpoint genOne (ctx: Ctx) (t: Typ) : G Expr :=
+  match t with
+  | TBool =>
+    b <- arbitrary ;;
+    ret (Bool b)
+  | TFun t1 t2 =>
+    t' <- genOne (t1 :: ctx) t2 ;;
+    ret (Abs t1 t')
+  end.
+
+
+Fixpoint genVar' (ctx: Ctx) (t: Typ) (p: nat) (r: list nat) : list nat :=
+  match ctx with
+  | nil => r
+  | t'::ctx' => if t == t' then genVar' ctx' t (p + 1) (p :: r)
+                else genVar' ctx' t (p + 1) r
+  end.
+
+
+Definition genVar (ctx: Ctx) (t: Typ) : list (G Expr) :=
+  let positions := genVar' ctx t 0 [] in
+  let tf := (fun n => ret (Var n)) in
+  map tf positions.
+
+
+Fixpoint genExactExpr (f: nat) (ctx: Ctx) (t: Typ) : G Expr :=
+  match f with
+  | O => oneOf_ (genOne ctx t) (genOne ctx t :: genVar ctx t)
+  | S f' =>
+    let abs : list (G Expr) := match t with
+              | TFun t1 t2 =>
+                [bindGen (genExactExpr f' (t1 :: ctx) t2) (fun t' => 
+                returnGen (Abs t1 t'))]
+              | _ => nil
+              end in
+    let one := genOne ctx t in
+    let app := 
+      t' <- genTyp f' ;;
+      e1 <- genExactExpr f' ctx (TFun t' t) ;;
+      e2 <- genExactExpr f' ctx t' ;;
+      ret (App e1 e2) in
+    let var := genVar ctx t in
+    
+    oneOf_ one ([one] ++ abs ++ [app] ++ var)
+  end.
+
+
+
+
+
+Definition genExpr (s: nat) : G Expr :=
+  t <- genTyp 3 ;;
+  genExactExpr s [] t
+.
+
+#[export] Instance arbitrarySizedExpr : GenSized Expr :=
+{|
+  arbitrarySized s := genExpr s
+|}.
+
+Definition gTyped := genExpr 5.
+
+Definition test_prop_SinglePreserve :=
+  forAll gTyped (fun (e: Expr) =>
+    prop_SinglePreserve e).
+
+(* QuickChick test_prop_SinglePreserve. *)
+
+Definition test_prop_MultiPreserve :=
+  forAll gTyped (fun (e: Expr) =>
+    prop_MultiPreserve e).
+
+(* QuickChick test_prop_MultiPreserve. *)
+
+
+
+
+
+
+*)
